% --------------------------------------------------------------------
% LaTeX Template for Math Homework
% --------------------------------------------------------------------

\documentclass{article}

% --- PACKAGE IMPORTS ---
% These packages add functionality for math symbols, formatting, etc.
\usepackage[margin=.7in]{geometry}       % For setting page margins
\usepackage{amsmath, amssymb, amsthm}   % American Mathematical Society packages for advanced math
\usepackage{graphicx}                   % For including images
\usepackage{fancyhdr}                   % For creating custom headers and footers
\usepackage[colorlinks=true, urlcolor=blue, linkcolor=blue]{hyperref} % For clickable links
\usepackage{cancel}
\usepackage{array}
\usepackage{amsfonts}
\usepackage{amsxtra}
\usepackage{epsfig}
\usepackage{wasysym}
\usepackage{relsize}
\usepackage{tikz}
\tikzset{every picture/.style={scale=1.2}}
\renewcommand{\normalsize}{\fontsize{12}{20}\selectfont}

% custom commands
\newcommand{\myauthor}{Miguel Gomez}
\newcommand{\canceling}[2]{\textcolor{red}{\cancelto{\textcolor{black}{#1}}{\textcolor{black}{#2}}}}
\newcommand{\todo}[1]{\textcolor{blue}{TODO:#1}}
% Save the original commands
\let\oldcos\cos
\let\oldsin\sin
\let\oldcosh\cosh
\let\oldsinh\sinh

% Redefine with automatic parentheses
\renewcommand{\cos}[1]{\oldcos\left(#1\right)}
\renewcommand{\sin}[1]{\oldsin\left(#1\right)}
\renewcommand{\cosh}[1]{\oldcosh\left(#1\right)}
\renewcommand{\sinh}[1]{\oldsinh\left(#1\right)}

\newcommand{\der}[2]{\frac{d#1}{d#2}}
\newcommand{\secder}[2]{\frac{d^2#1}{d#2^2}}
\newcommand{\parder}[2]{\frac{\partial#1}{\partial#2}}
\newcommand{\secparder}[2]{\frac{\partial^2#1}{\partial#2^2}}

% --- DOCUMENT & AUTHOR INFORMATION ---
\title{Homework \#5}
\author{
	MATH 3160 -- Complex Variables\\
	\myauthor
}
\date{Completed: \today}

% --- HEADER & FOOTER CONFIGURATION ---
% This section sets up the header that will appear on each page.
\pagestyle{fancy}
\fancyhf{} % Clears the default header and footer
\lhead{Math 3160 -- HW \# 5} % Left side of header
\rhead{\myauthor} % Puts the author's name on the right side
\rfoot{Page \thepage} % Puts the page number on the bottom right

\begin{document}

\maketitle % This command generates the title based on the information above.

% ====================================================================
% --- START OF PROBLEMS ---
% ====================================================================

\section*{Problem 1}
Consider the analytic function $f(z) = z e^{z^2}$.
\begin{enumerate}
	\item [(a)] Show that the function $u(x,y) = x \ e^{(x^2 - y^2)} \cos{2xy} - y \ e^{(x^2 - y^2)} \sin{2xy}$ is the real component of $f(z)$.
	\item [(b)] What is a harmonic conjugate for $u(x,y)$?
	\item [(c)] Without computing the second partial derivatives of $u(x,y)$, explain why you know that $u(x,y)$ is harmonic.
\end{enumerate}

\vspace{.5cm} % Space between problems

\hrule % Adds a horizontal line to separate problems.
Expanding $f(z) = z e^{z^2}$ to see what the $u$ and $v$ turn out to be.
\subsection*{(a)}
\begin{align*}
  f(z) &= z e^{z^2} = (x+iy)e^{(x+iy)^2} = (x+iy)e^{x^2-y^2+2ixy} = (x+iy)e^{x^2-y^2}e^{2ixy}\\
  &= e^{x^2-y^2}(x+iy)(\cos{2xy}+i\sin{2xy}) \\
       &= e^{x^2-y^2}(x\cos{2xy}+ix\sin{2xy} + iy\cos{2xy}+i^2y\sin{2xy})\\
       &=  e^{x^2-y^2}(x\cos{2xy}-y\sin{2xy} + i(x\sin{2xy} + y\cos{2xy}))\\
       &\therefore u(x,y) = e^{x^2-y^2}(x\cos{2xy}-y\sin{2xy})
\end{align*}
\subsection{(b)}
Utilizing the imaginary part of $f$, $v$ can serve as a conjugate up to an arbitrary constant, which we could set to 0 to recover $f$. 
\begin{align*}
v(x,y) &= e^{x^2-y^2} (x\sin{2xy} + y\cos{2xy}) + C
\end{align*}
\subsection{(c)}
Since we know that $f$ is analytic as stated, and $u$ is the real part of $f$, an analytic function, then $u$ must be harmonic. This is due to the fact that the real and imaginary parts of any analytic function are harmonic functions.
\newpage
\section*{Problem 2}
Consider the function  $u(x,y) = x^3 - 3 x y^2 - 3 x^2 y + y^3$.

\begin{enumerate}
	\item [(a)] Show that $u(x,y)$ is harmonic.
	\item [(b)] Find a harmonic conjugate for $u(x,y)$.
\end{enumerate}


\vspace{.5cm} % Space between problems

\hrule
\subsection*{(a)}
For this, we can start by showing that the expression for $u$ satisfies the Laplacian:
\begin{align*}
  \secparder{u}{x} &+ \secparder{u}{y} = 0\\
  \parder{u}{x} &= 3x^2 - 3 y^2 - 6xy\\
  \secparder{u}{x} &= 6x - 6y\\
  \parder{u}{y} &= - 6 x y - 3 x^2  + 3y^2\\
  \secparder{u}{y} &= - 6 x  + 6y\\
  \secparder{u}{x} &+ \secparder{u}{y} = 6x - 6y + (- 6 x  + 6y) = 0\\
  \therefore &\ u(x,y)\ \text{is harmonic.}
\end{align*}
\subsection*{(b)}
For a conjugate, we can back solve to get the $v$ expression that works.
\begin{align*}
  \parder{u}{x} &= \parder{v}{y} \\
  v(x,y) = \int 3x^2 - 3 y^2 - 6xy dy &= 3x^2y - y^3 - 3xy^2 + G(x)\\
  \parder{u}{y} &= -\parder{v}{x} \\
  v(x,y) = \int  6 x y + 3 x^2  - 3y^2 dx &= 3x^2y + x^3 -3x^2y + G(y)\\
  \therefore  v(x,y)_1 &= v(x,y)_2 \\
  G(x) &= x^3 + C\\
  G(y) &= -y^3 + C\\
  \therefore v(x,y) &= \boxed{ 3x^2y + x^3 -3x^2y + -y^3 + C}
\end{align*}
\newpage
\section*{Problem 3}
Recall we learned of the following fact in class:

\begin{center}
	{\em Let $u(x,y)$ be a harmonic function defined on a simply connected domain $D$. \\ Then $u(x,y)$ has a harmonic conjugate on $D$.}
\end{center}

\begin{enumerate}
	\item [(a)] Show that $u(x,y) = \ln(\sqrt{x^2 + y^2})$ is a harmonic function.

	\item [(b)] What is the domain of definition of $u(x,y)$?

	\item [(c)] An aside: show that if $f(z)$ and $g(z)$ are two analytic functions on the same domain $D$, and we have $\text{Re}(f(z)) = \text{Re}(g(z))$ for all $z \in D$, then $f(z) = g(z) + c$ for some constant $c \in \mathbb{C}$.

          [{\em Hint: show that the function $h(z) = f(z) - g(z)$ has $\text{Re}(h(z)) = 0$, and then use a result from class to conclude $h(z)$ is a constant.}]

	\item [(d)] Explain why $u(x,y)$ does {\it not} have a harmonic conjugate on its domain.

          [{\em Hint: if such a conjugate existed, then $u(x,y)$ would be the real component of some analytic function $f(z)$, but $u(x,y)$ is already the real component of a familiar analytic function, which is discontinuous at its branch cut}]

	\item Why does this not contradict the fact from class?
\end{enumerate}

\vspace{.5cm} % Space for work

\hrule
\subsection*{(a)}
\begin{align*}
  u(T) = \ln(T),\ \ T(S) &= \sqrt{S}, \ \ S = x^2+y^2 \\ 
  \der{u}{T} = \frac{1}{T} \ \ \der{T}{S} &= \frac{1}{2\sqrt{S}}\ \ \parder{S}{x|y} = 2x|2y\\
  \parder{u}{x} = \parder{}{x}(\ln{((x^2+y^2)^{\frac{1}{2}})}) &= ((x^2+y^2)^{-\frac{1}{2}})\left(\frac{1}{2}(x^2+y^2)^{-\frac{1}{2}}\right)(2x) \\
  &=\left(\frac{2x}{2(x^2+y^2)}\right)\\
  \parder{u}{x} &=\left(\frac{x}{x^2+y^2}\right)\\
  \parder{u}{y} &= \left(\frac{y}{x^2+y^2}\right)
\end{align*}
\begin{align*}
  \secparder{u}{x} =\frac{f'g-fg'}{g^2} &= \left(\frac{(x)'(x^2+y^2)-(x)(x^2+y^2)'}{(x^2+y^2)^2}\right)\\
                                        &= \left(\frac{(x^2+y^2)-(x)(2x)}{(x^2+y^2)^2}\right)\\
  \secparder{u}{x} &= \left(\frac{(y^2-x^2)}{(x^2+y^2)^2}\right)\\
  \secparder{u}{y}&= \left(\frac{(x^2-y^2)}{(x^2+y^2)^2}\right)\\
  \secparder{u}{x} &+ \secparder{u}{y} =  \frac{y^2-x^2 + x^2-y^2}{(x^2+y^2)^2} = 0
\end{align*}
\subsection*{(b)}
\begin{align*}
  \ln{(\sqrt{x^2+y^2})} &= \frac{1}{2}\ln{(x^2+y^2)} = \frac{1}{2}\ln{(|z|)}
\end{align*}
Domain of definition is anywhere that the magnitude is not zero.
\begin{align*}
  \mathbb{C}\setminus \{0\}
\end{align*}
\subsection*{(c)}
\subsection*{(d)}
It does not because it is a function that has a behavior that exhibits periodicity due to the arg$(z)$. Because of this, the answers repeat for integer values $k$. The inclusion of the branch cut means that it cannot be continuous across branch cuts.
\newpage
\section*{Problem 4}
Find the following values, on the branches given:
\begin{enumerate}
	\item [(a)] $ \log(3) \ \ (-2\pi \leq \theta < 0)$ 
	\item [(b)] $ \log(-1 + i) \ \ (-\pi/2 < \theta \leq 3 \pi / 2)$
	\item [(c)] $ \log(1 - i \sqrt 3) \ \ (\pi \leq \theta < 3 \pi)$.
\end{enumerate}
\hrule
\vspace{.5cm} % Space for work

\begin{align*}
  \log(z) &= \log{|z|} + iarg(z) = \log{|z|} + i(Arg(z) + 2\pi k)\ \forall k \in \mathbb{Z}
\end{align*}
\subsection*{(a)}
$ \log{(3)} \ \ (-2\pi \leq \theta < 0)$
\begin{align*}
  \log{(3)} &=  \log{|3|} + i(Arg(3) + 2\pi k)= \log{(3)} + i(0 +  2\pi k)\\
  \log{(3)} &+ i(2\pi k)\ k \in [-1,0) \quad \k = -1\\
  &= \log{(3)} - i2\pi
\end{align*}
\subsection*{(b)}
$ \log(-1 + i) \ \ (-\pi/2 < \theta \leq 3 \pi / 2)$
\begin{align*}
  \log{(-1 + i)} &=  \log{|-1 + i|} + i(Arg(-1 + i) + 2\pi k)= \log{(\sqrt{2})} + i\left(\frac{3\pi}{4} +  2\pi k\right)\\
  \log{(\sqrt{2})} &+ i\left(\frac{3\pi}{4}+2\pi k\right)\ k \in \left(-\frac{1}{4}, \frac{3}{4}\right]\\
                 &= \log{(\sqrt{2})} + i\left(\frac{3\pi}{4}+2\pi k\right) \ k = 0\\
                 &= \log{(\sqrt{2})} + i\frac{3\pi}{4}
\end{align*}
\subsection*{(c)}
$ \log(1 - i \sqrt 3) \ \ (\pi \leq \theta < 3 \pi)$
\begin{align*}
  \log{(1-i\sqrt{3})} &=  \log{|1-i\sqrt{3}|} + i(Arg(1-i\sqrt{3}) + 2\pi k)= \log{(2)} - i\left(\frac{\pi}{3} +  2\pi k\right)\\
  &= \log{(2)} - i\left(\frac{\pi}{3} +  2\pi k\right) \ k\in \left[\frac{1}{2},\frac{3}{2}\right) \quad k = 1\\
  &= \log{(2)} +i\frac{5\pi}{3} 
\end{align*}
\newpage
\section*{Problem 5}
Recall that power functions are defined by $z^c = e^{c \log(z)}$. In this exercise, we compute all power functions by using the branch $(0 \leq \theta < 2 \pi)$ for $\log(z)$.
\begin{enumerate}
	\item [(a)] For $z = -i$ and $c = i$, compute the values of $(z^c)^2$, $(z^2)^c$, and $z^{(2c)}$.
	\item [(b)] With the notation as in (a), which of these are true or false?
	      $$ (z^c)^2 = (z^2)^c, \hspace{20pt} (z^c)^2 = z^{(2c)}, \hspace{20pt} (z^2)^c = z^{(2c)}.$$

\end{enumerate}

\end{document}

%%% Local Variables:
%%% mode: latex
%%% TeX-master: t
%%% End:





